src/Extraction.v
@@ -9,7 +9,7 @@ Extraction Language Haskell.
 Cd "extraction/src".
 
 Extract Inductive bool => "Prelude.Bool" ["Prelude.True" "Prelude.False"].
-Extract Inductive sumbool => "Prelude.Either" ["Prelude.Left" "Prelude.Right"].
+Extract Inductive sumbool => "Prelude.Bool" ["Prelude.True" "Prelude.False"].
 Extract Inductive list => "[]" [ "[]" "(:)" ].
 Extract Inductive prod => "(,)"  [ "(,)" ].
 Extract Inductive sumorT => "Prelude.Either" ["Prelude.Left" "Prelude.Right"].
